theories/ValueOpts/ConstantPropagationAnalysisCorrect.v
@@ -1,0 +1,87 @@
+Require Import Util SizeInduction Get.
+Require Import AnalysisForwardSSA Subterm CSet MapAgreement RenamedApart.
+Require Import Infra.PartialOrder Infra.Lattice Infra.WithTop.
+Require Import LabelsDefined Annotation.
+Require Import ConstantPropagation ConstantPropagationAnalysis.
+
+Local Arguments proj1_sig {A} {P} e.
+Local Arguments length {A} e.
+Local Arguments forward {sT} {Dom} {H} {H0} {H1} ftransform ZL st ST d.
+
+Lemma option_R_inv x y
+  : @OptionR.option_R (withTop Val.val) (withTop Val.val)
+         (@poEq (withTop Val.val)
+                (@withTop_PO Val.val Val.int_eq Val.Equivalence_eq_int' Val.int_eq_dec)) x y
+    -> x = y.
+Proof.
+  intros. inv H; eauto.
+  inv H0; eauto.
+  do 2 f_equal. eauto.
+Qed.
+
+
+Lemma cp_forward_agree sT ZL AE G s (ST:subTerm s sT) ra
+  (RA:renamedApart s ra)
+  : agree_on poLe (G \ snd (getAnn ra))
+             (domenv AE)
+             (domenv (forward constant_propagation_transform ZL s ST AE)).
+Proof.
+  general induction RA; simpl in *.
+  - destruct e.
+    + pose proof (IHRA sT ZL (domupd AE x (op_eval (domenv AE) e)) G
+                       (subTerm_EQ_Let eq_refl ST)); eauto.
+      pe_rewrite. set_simpl.
+      etransitivity; eauto.
+      eapply agree_on_incl; eauto with cset.
+      hnf; intros.
+      unfold domupd, domenv; simpl.
+      cases; lud; cset_tac'; reflexivity.
+    + pose proof (IHRA sT ZL (domupd AE x (Some Top)) G
+                       (subTerm_EQ_Let eq_refl ST)); eauto.
+      pe_rewrite. set_simpl.
+      etransitivity; eauto.
+      eapply agree_on_incl; eauto with cset.
+      hnf; intros.
+      unfold domupd, domenv; simpl.
+      lud; cset_tac'; reflexivity.
+  - pe_rewrite. set_simpl.
+    repeat cases; eauto using agree_on_incl with cset.
+    + admit.
+    + admit.
+  - reflexivity.
+  - admit.
+
+Qed.
+
+Definition cp_sound sT AE Cp ZL s (ST:subTerm s sT)
+  : poEq (forward constant_propagation_transform ZL s ST AE) AE
+    -> labelsDefined s (length ZL)
+    -> cp_sound (domenv AE) Cp s.
+Proof.
+  intros EQ LD.
+  general induction LD; simpl in *.
+  - destruct e; simpl.
+    + specialize (EQ x).
+      admit.
+
+    + econstructor; eauto.
+      simpl. admit.
+  - let_case_eq; try let_pair_case_eq; subst; simpl in *;
+      repeat cases in EQ; simpl in *;
+        econstructor; intros; eauto;
+          try rewrite COND in *; simpl in *;
+            try rewrite Val.val2bool_true in *;
+            try rewrite Val.val2bool_false in *;
+            isabsurd.
+    + admit.
+    + admit.
+    + eapply IHLD1; eauto. admit.
+    + eapply IHLD2; eauto. admit.
+  - econstructor.
+  - (* invariant with ZL and Cp *) admit.
+  - econstructor.
+    + intros.
+      eapply H0 with (ZL0:=fst ⊝ F ++ ZL); eauto with len.
+      admit.
+    + eapply IHLD with (ZL0:=fst ⊝ F ++ ZL); eauto with len.
+Admitted.
